# Calculations

```m
z=tf('z',1/Fs);
DL1=(z)^-(M-i0);
DL2=(z)^-(i0);
Hl=gl*(1+al)/(1+al*z^-1);
Hd=(ad+z^-1)/(1+ad*z^-1);
```

```m
z=tf('z',1/Fs);
```
$$
f(z) = z
$$
$$
f(z) = \frac{z}{1}
$$
$$
f(z) = \frac{z^1}{z^0}
$$

```m
M=38;
i0=5;
DL1=(z)^-(M-i0);
```

$$
f(z) = 1.0 / z^{33}
$$
$$
f(z) = \frac{1}{z^{33}}
$$
$$
f(z) = \frac{z^0}{z^{33}}
$$

```m
DL1=(z)^-(i0);
```
$$
f(z) = 1.0 / z^{5}
$$
$$
f(z) = \frac{1}{z^{5}}
$$
$$
f(z) = \frac{z^0}{z^{5}}
$$

```m
gl=-0.99;
al= -0.001;
Hl=gl*(1+al)/(1+al*z^-1);
```

$$
f(z) = -0.99*(1 + -0.001) / (1 + -0.001*({\frac{z^1}{z^0}})^{-1})
$$
$$
f(z) = -0.99*(1 + -0.001) / (1 + -0.001*{\frac{z^0}{z^1}})
$$
$$
f(z) = -0.989 / (1 + -0.001*{\frac{z^0}{z^1}})
$$
$$
f(z) = -0.989 / (1 + {\frac{-0.001*z^0}{z^1}})
$$
$$
f(z) = -0.989 / (\frac{z^1}{z^1} + {\frac{-0.001*z^0}{z^1}})
$$
$$
f(z) = -0.989 / \frac{z^1 +-0.001*z^0}{z^1}
$$
$$
f(z) = -0.989 * \frac{z^1}{ z^1 +-0.001*z^0}
$$
$$
f(z) = \frac{-0.989*z^1}{ 1*z^1 +-0.001*z^0}
$$

Result
$$
f(z) = \frac{-0.98901*z}{-0.001 +z}
$$
---
$$
f(z) = \\frac{-0.98901*z^{14} +3.881073041999999*z^{15} -7.029012751199999*z^{16} +7.779303429479999*z^{17} -5.8700196244799985*z^{18} +3.189003305498999*z^{19} -1.2832784055115196*z^{20} +0.3872866466470319*z^{21} -0.08765769861913678*z^{22} +0.014695983623781895*z^{23} -0.0017738820973249195*z^{24} +0.0001459837767105828*z^{25} -0.000007341587272910878*z^{26} +0.00000017039967023752195*z^{27}}{ 0.00000000017229317219999994*z^{13} -0.00000017971634008799996*z^{14} +0.000007570773854279998*z^{15} -0.000149399559972*z^{16} +0.0018084529791899994*z^{17} -0.014947918951679996*z^{18} +0.08902335190319997*z^{19} -0.3928877615519999*z^{20} +1.3007627918999995*z^{21} -3.2303751479999994*z^{22} +5.943113747999998*z^{23} -7.872855119999999*z^{24} +7.1110441999999985*z^{25} -3.925199999999999*z^{26} +z^{27}}"
$$